Strong stepping

src/lang1.v
@@ -1,6 +1,5 @@
 From iris.program_logic Require Export language ectx_language ectxi_language.
 From cbpv Require Import base syntax semantics.
-
 Definition of_val (n : nat) (v : value n) : comp n := ret v.
 
 Definition to_val (n : nat) (c : comp n) : option (value n) :=
@@ -10,31 +9,59 @@ Definition to_val (n : nat) (c : comp n) : option (value n) :=
   end.
 
 Variant head_step {n : nat} : comp n -> unit -> list unit -> comp n -> unit -> list (comp n) -> Prop :=
-| cstep_step c1 c2 : cstep c1 c2 ->
+| strong_head_step c1 c2 : strong_step c1 c2 ->
                      head_step c1 tt nil c2 tt nil.
 
-
-Lemma Inj_fill n:
-  ∀ Ki : ectx, Inj eq eq (@fill n Ki).
+Lemma Inj_fill_vctx n m:
+  ∀ Ki : cctx false n m, Inj eq eq (@fillc n _ _ Ki).
 Proof.
-  intros. induction Ki; repeat intro; auto; inv H; apply IHKi; auto.
+  revert n m.
+  eapply mutind_vctx_cctx; cbn; exintuition.
+  all : repeat intro; intuition ; try contradiction.
+  all : match goal with
+  | [ IH: Inj _ _ _ , H : _ = _ |- _] => eapply IH; inv H; eauto
+  end.
 Qed.
 
 Lemma to_of_val n v : to_val n (of_val n v) = Some v.
-  Proof. by induction v; simplify_option_eq. Qed.
+Proof. by induction v; try simplify_option_eq. Qed.
 
-
-Lemma lang_mixin n : EctxiLanguageMixin (of_val n) (to_val n) fill head_step.
+Require Import Coq.Program.Equality.
+Lemma lang_mixin n : EctxiLanguageMixin (of_val n) (to_val n) (fillc (t := false)) head_step.
 Proof.
   split; auto.
   - unfold of_val, to_val. intros. destruct e; inversion H; auto.
-  - intros. inversion H. subst. inversion H0. subst. inv H1; destruct C; simpl; auto.
-  - intros. destruct Ki; simpl in *; auto; try inv H; inv H0.
+  - intros. inv H. inv H0.
+    (* revert n m c1 K c2 H. eapply mutind_vctx_cctx; cbn; intuition. *)
+    (* all : repeat intro; intuiition; *)
+    (* destruct K; eauto. clear H. destruct y. *)
+    (* cbn.  *)
+  (* destruct K; simpl; eauto. inv y. eauto. inv H; destruct K; simpl; auto.  exintuition. *)
+    admit.
+  - revert n.
+    (* eapply mutind_vctx_cctx; cbn; exintuition. *)
+    (* Unshelve. 5 : exact false. *)
+    admit.
+    (* eauto.  *)
+
+    (* dependent induction Ki. *)
+    (* 1-3: intros; eauto.  cbn in H; try solve [inv H; inv H0]. *)
+    (* revert e H. *)
+    (* dependent induction v. inv y. *)
+    (* all : intros; try eapply IHv; eauto. *)
+
+    (* eapply  *)
+
+  (* inv H. inv H0.  *)
+
+
+
   - apply Inj_fill.
   - induction Ki1, Ki2; intros; try discriminate; simplify_eq;
     repeat match goal with
            | H : to_val (of_val _) = None |- _ => by rewrite to_of_val in H
            end; auto.
+
     eapply IHKi1 in H1; subst; eauto.
     eapply IHKi1 in H2; subst; eauto.
     eapply IHKi1 in H1; subst; eauto.
@@ -44,3 +71,5 @@ Proof.
   split; apply _ || eauto using to_of_val, of_to_val, val_head_stuck,
          fill_item_.,`val, fill_item_no_val_inj, head_ctx_step_val.
 Qed.
+
+EctxiLanguageMixin
